Mincost_Flow_Algorithms/Use_Orlins_Algorithm/Usage_Multigraph.thy
@@ -7,11 +7,13 @@ begin
 datatype 'a edge_type = an_edge "('a \<times>'a)" | another_edge "('a \<times> 'a)"
 
 definition "create_edge x y = an_edge (x,y)"
-fun make_pair where
- "make_pair (an_edge e) = e"|
- "make_pair (another_edge e) = e"
+fun fstt where
+ "fstt (an_edge e) = fst e"|
+ "fstt (another_edge e) = fst e"
 
-  
+fun sndd where
+ "sndd (an_edge e) =snd e"|
+ "sndd (another_edge e) = snd e" 
   instantiation edge_type::(linorder) linorder
 begin
 
@@ -138,21 +140,10 @@ value "dfs_impl G 9 (dfs_initial_state 0)"
 value "vset_diff (nbs edges (1::nat)) (nbs edges (2::nat))"
 end
 
-context begin
-value "lookup G 1"
-value "lookup G 12"
-value "lookup' (Replace G) 12"
-value "lookup' (Replace G) 1"
-value "lookup' (edge_map_update' 1 (list_to_rbt [1::nat,2,3,4,5,6,7,8]) (Replace G)) 100"
-value "remove_all_empties (edge_map_update' 1 (list_to_rbt [1::nat,2,3,4,5,6,7,8]) (Replace G))"
-value "lookup (remove_all_empties (edge_map_update' 1 (list_to_rbt [1::nat,2,3,4,5,6,7,8]) (Replace G))) 100"
-end
-
-
-definition "final_state_multi = final_state make_pair create_edge \<E>_impl \<c>_impl \<b>_impl flow_lookup"
+definition "final_state_multi = final_state fstt sndd create_edge \<E>_impl \<c>_impl \<b>_impl flow_lookup"
 value final_state_multi
 
-definition "final_flow_impl_multi =  final_flow_impl make_pair create_edge \<E>_impl \<c>_impl \<b>_impl flow_lookup"
+definition "final_flow_impl_multi =  final_flow_impl fstt sndd create_edge \<E>_impl \<c>_impl \<b>_impl flow_lookup"
 value final_flow_impl_multi
 
 definition "final_forest = (\<FF> final_state_multi)"
@@ -162,7 +153,8 @@ value "map (\<lambda> (x, y). (x, inorder y)) (inorder final_forest)"
 value "inorder (conv_to_rdg final_state_multi)"
 value "inorder (not_blocked final_state_multi)"
 
-lemma no_cycle: "closed_w (make_pair ` \<E> \<E>_impl) (map make_pair C) \<Longrightarrow> (set C \<subseteq> \<E> \<E>_impl) \<Longrightarrow>
+lemma no_cycle: "closed_w (make_pair fstt sndd ` \<E> \<E>_impl) (map (make_pair fstt sndd) C)
+          \<Longrightarrow> (set C \<subseteq> \<E> \<E>_impl) \<Longrightarrow>
         foldr (\<lambda>e acc. acc + \<c> \<c>_impl flow_lookup e) C 0 < 0 \<Longrightarrow> False"
 proof(goal_cases)
   case 1
@@ -197,51 +189,43 @@ next
     by(auto simp add: \<E>_impl_def set_invar_def selection_functions.\<E>_def to_set_def)
 qed
 
-lemma multigraph: "multigraph (prod.fst o make_pair) (prod.snd o  make_pair) make_pair create_edge (\<E> \<E>_impl)"
-  apply(rule multigraph.intro)
-  subgoal for e x y
-    by(cases e) auto
-  subgoal for x y
-    by (simp add: create_edge_def)
-   apply (simp add: \<E>_impl_basic(3))
-  using selection_functions.\<E>_def \<E>_impl_basic(2) by blast
+lemma multigraph: "multigraph fstt sndd create_edge (\<E> \<E>_impl)"
+  using \<E>_impl_basic(2,3)
+  by(auto intro!: multigraph.intro simp add: create_edge_def  selection_functions.\<E>_def)
 
+lemma Vs_is: "dVs (make_pair fstt sndd ` to_set \<E>_impl) = {1,2,3,4,5,6}"
+  unfolding to_set_def \<E>_impl_def 
+  by (auto simp add: dVs_def make_pair_def multigraph_spec.make_pair_def)
 
-lemma Vs_is: "dVs (make_pair ` to_set \<E>_impl) = {1,2,3,4,5,6}"
-  unfolding to_set_def \<E>_impl_def by (auto simp add: dVs_def)
-
-lemma Vs_is_bal_dom: "dVs (make_pair ` to_set \<E>_impl) = dom (bal_lookup \<b>_impl)" 
-  apply(rule trans[of  _ "{1,2,3,4,5,6}"])
-  subgoal
-  unfolding to_set_def \<E>_impl_def by (auto simp add: dVs_def)
-  subgoal
-    unfolding dom_def bal_lookup_def \<b>_impl_def update_def b_list_def
-    by auto
-  done
+lemma Vs_is_bal_dom: "dVs (make_pair fstt sndd` to_set \<E>_impl) = dom (bal_lookup \<b>_impl)" 
+  apply(rule trans[OF Vs_is])
+  by(auto simp add: dom_def bal_lookup_def \<b>_impl_def update_def b_list_def)
                 
-lemma at_least_2_verts:" 1 < function_generation.N \<E>_impl to_list (prod.fst o make_pair) (prod.snd o make_pair)"
+lemma at_least_2_verts:" 1 < function_generation.N \<E>_impl to_list fstt sndd"
   apply(subst function_generation.N_def[OF selection_functions.function_generation_axioms])
   by(auto simp add: to_list_def \<E>_impl_def)
 
-lemma no_cycle_cond: "no_cycle_cond make_pair \<c>_impl \<E>_impl flow_lookup" 
-  by (metis \<E>_def \<c>_def no_cycle no_cycle_cond_def)
+lemma no_cycle_cond: "no_cycle_cond fstt sndd \<c>_impl \<E>_impl flow_lookup" 
+  using no_cycle
+  by(auto simp add: no_cycle_cond_def \<c>_def make_pair_def \<E>_def) 
 
-lemma correctness_of_algo:"correctness_of_algo make_pair \<E>_impl create_edge \<b>_impl"
-  using \<E>_impl_basic at_least_2_verts gt_zero multigraph
-  by (auto intro!: correctness_of_algo.intro simp add: \<b>_impl_def bal_invar_b Vs_is_bal_dom  \<E>_def)
- 
+lemma correctness_of_algo:"correctness_of_algo fstt sndd \<E>_impl create_edge \<b>_impl"
+  using \<E>_impl_basic at_least_2_verts gt_zero multigraph Vs_is_bal_dom
+  by (auto intro!: correctness_of_algo.intro 
+         simp add: \<b>_impl_def bal_invar_b Vs_is_bal_dom  \<E>_def make_pair_def)
+
 corollary correctness_of_implementation:
  "return final_state_multi = success \<Longrightarrow>  
-        cost_flow_spec.is_Opt (fst o make_pair) (snd o make_pair) make_pair \<u> (\<E> \<E>_impl) (\<c> \<c>_impl flow_lookup) (\<b> \<b>_impl) 
+        cost_flow_spec.is_Opt fstt sndd \<u> (\<E> \<E>_impl) (\<c> \<c>_impl flow_lookup) (\<b> \<b>_impl) 
  (abstract_flow_map final_flow_impl_multi)"
  "return final_state_multi = failure \<Longrightarrow> 
-         \<nexists> f. flow_network_spec.isbflow  (fst o make_pair) (snd o make_pair) make_pair (\<E> \<E>_impl) \<u>  f (\<b> \<b>_impl)"
+         \<nexists> f. flow_network_spec.isbflow  fstt sndd (\<E> \<E>_impl) \<u>  f (\<b> \<b>_impl)"
  "return final_state_multi = notyetterm \<Longrightarrow>  
          False"
   using correctness_of_algo.correctness_of_implementation[OF correctness_of_algo no_cycle_cond]
   by(auto simp add: final_state_multi_def final_flow_impl_multi_def)
 
-lemma opt_flow_found: "cost_flow_spec.is_Opt (fst o make_pair) (snd o make_pair) make_pair \<u>  (\<E> \<E>_impl) (\<c> \<c>_impl flow_lookup) (\<b> \<b>_impl)  (abstract_flow_map final_flow_impl_multi)"
+lemma opt_flow_found: "cost_flow_spec.is_Opt fstt sndd \<u>  (\<E> \<E>_impl) (\<c> \<c>_impl flow_lookup) (\<b> \<b>_impl)  (abstract_flow_map final_flow_impl_multi)"
   apply(rule correctness_of_implementation(1))
   by eval
 end
