Mincost_Flow_Algorithms/Use_Orlins_Algorithm/Existence_Optflows.thy
@@ -50,21 +50,14 @@ lemma \<u>_impl_props: "dom (flow_lookup \<u>_impl) = \<E>" "(\<forall> e \<in> 
   using  u_impl_exists[simplified sym[OF some_eq_ex]] 
   by (auto simp add: \<u>_impl_def) 
 
-thm with_capacity_proofs.correctness_of_implementation[of _ _ _ make_pair create_edge _ _ \<E> \<u> \<c> ]
+thm with_capacity_proofs.correctness_of_implementation[of  snd _ _ _ fst create_edge _ _ \<E> \<u> \<c> ]
 
-lemma cost_flow_network_impl:"cost_flow_network (prod.fst \<circ> make_pair) (prod.snd \<circ> make_pair) make_pair create_edge (the_default PInfty \<circ> flow_lookup \<u>_impl) \<E>"
-proof -
-  have "snd = prod.snd \<circ> make_pair \<and> fst = prod.fst \<circ> make_pair"
-    by (auto simp add: make_pair''(1) make_pair''(2))
-  then show "cost_flow_network (prod.fst \<circ> make_pair) (prod.snd \<circ> make_pair) make_pair create_edge (the_default PInfty \<circ> flow_lookup \<u>_impl) \<E>"
-    using cost_flow_network_axioms \<u>_impl_props(1,2)
+lemma cost_flow_network_impl:"cost_flow_network fst snd create_edge (the_default PInfty \<circ> flow_lookup \<u>_impl) \<E>"
+ using cost_flow_network_axioms \<u>_impl_props(1,2)
     by(force split: option.split simp add: cost_flow_network_def flow_network_def flow_network_axioms_def the_default_def 
                      dom_def)
-qed
 
-lemma cost_flow_network2:"flow_network (prod.fst \<circ> make_pair) (prod.snd \<circ> make_pair) make_pair create_edge \<u> \<E>"
-  using finite_E  by(auto intro!: flow_network.intro multigraph.intro flow_network_axioms.intro 
-                           simp add: create_edge E_not_empty u_non_neg)
+lemmas cost_flow_network2 = flow_network_axioms
 
 lemma b_impl_exists: "\<exists> b_impl. dom (bal_lookup b_impl) = \<V>  \<and> 
                          (\<forall> v \<in> \<V>. bal_lookup b_impl v = Some (b v)) \<and> bal_invar b_impl"
@@ -91,7 +84,7 @@ lemma b_impl_props: "dom (bal_lookup (b_impl b)) = \<V> " "(\<forall> v \<in> \<
   using  b_impl_exists[simplified sym[OF some_eq_ex]] 
   by (auto simp add: b_impl_def) force
 
-lemma with_capacity_proofs: "with_capacity_proofs \<c>_impl (b_impl b) c_lookup make_pair create_edge \<E>_impl \<u>_impl \<E> 
+lemma with_capacity_proofs: "with_capacity_proofs snd \<c>_impl (b_impl b) c_lookup fst  create_edge \<E>_impl \<u>_impl \<E> 
 (the_default PInfty \<circ> flow_lookup \<u>_impl) \<c> (the_default 0 \<circ> bal_lookup (b_impl b))"
   apply(rule with_capacity_proofs.intro[OF cost_flow_network_impl], rule with_capacity_proofs_axioms.intro)
   using b_impl_props[of b]
@@ -100,15 +93,14 @@ lemma with_capacity_proofs: "with_capacity_proofs \<c>_impl (b_impl b) c_lookup 
 
 interpretation algo_locale: with_capacity_proofs
   where \<c>_impl = \<c>_impl and \<b>_impl = "(b_impl b)" 
-  and c_lookup = c_lookup and make_pair = make_pair and create_edge = create_edge
+  and c_lookup = c_lookup and fst = fst and snd = snd and create_edge = create_edge
   and \<E>_impl = \<E>_impl and \<u>_impl = \<u>_impl and \<E> = \<E>
   and \<u> = "the_default PInfty \<circ> flow_lookup \<u>_impl" and \<c> = \<c>
  and \<b> = "the_default 0 \<circ> bal_lookup (b_impl b)"
   using with_capacity_proofs by simp
 
 lemma algo_locale_isbflow_def:"algo_locale.isbflow f b = flow_network_spec.isbflow
-                               (prod.fst o make_pair) (prod.snd o make_pair)
-                                 make_pair \<E> (the_default PInfty \<circ> flow_lookup \<u>_impl) f b"
+                               fst snd \<E> (the_default PInfty \<circ> flow_lookup \<u>_impl) f b"
   by auto
 thm algo_locale.correctness_of_implementation
 
@@ -129,7 +121,7 @@ proof(rule, goal_cases)
       using 1(1) 
       by (auto simp add: Min_gr_iff Rcap_def)
     have same_path:"(map (to_vertex_pair \<circ> F) D) = (map make_pair D)" 
-      by simp
+      by (simp add: make_pair_def Instantiation.make_pair_def)
     have fstv_is: "fstv (hd (map F D)) = u"
       using u_prop(2) awalk_hd[OF u_prop(1)]
       by(cases D)(auto simp add:  make_pair'')
@@ -186,17 +178,17 @@ next
     using no_neg_cycle \<u>_impl_props(1,2) 
     by(force simp add: the_default_def) 
   have an_opt:"algo_locale.is_Opt (the_default 0 \<circ> bal_lookup (b_impl b))
-   (abstract_flow_map (with_capacity.final_flow_impl_original make_pair \<E>_impl \<c>_impl \<u>_impl (b_impl b) c_lookup))"
+   (abstract_flow_map (with_capacity.final_flow_impl_original fst snd \<E>_impl \<c>_impl \<u>_impl (b_impl b) c_lookup))"
     using  algo_locale.correctness_of_implementation[OF no_neg_cycle'] a_flow 
            return.exhaust by blast
   have another_opt:"is_Opt (the_default 0 \<circ> bal_lookup (b_impl b))
-   (abstract_flow_map (with_capacity.final_flow_impl_original make_pair \<E>_impl \<c>_impl \<u>_impl (b_impl b) c_lookup))"
+   (abstract_flow_map (with_capacity.final_flow_impl_original fst snd \<E>_impl \<c>_impl \<u>_impl (b_impl b) c_lookup))"
     using  cost_flow_network_axioms  \<u>_impl_props 
     by(subst comp_def) 
       (force intro!: capacity_Opt_cong[OF cost_flow_network_impl _ _ an_opt, of \<u>, simplified comp_def make_pair'' ] 
            simp add: the_default_def)
    have "is_Opt b
-   (abstract_flow_map (with_capacity.final_flow_impl_original make_pair \<E>_impl \<c>_impl \<u>_impl (b_impl b) c_lookup))"
+   (abstract_flow_map (with_capacity.final_flow_impl_original fst snd \<E>_impl \<c>_impl \<u>_impl (b_impl b) c_lookup))"
      using b_impl_props(1)
      by(auto intro!: is_Opt_cong[OF refl _  another_opt] simp add: the_default_def b_impl_props(2) split: option.split)     
    then show ?case 
@@ -254,18 +246,14 @@ lemma \<u>_impl_props: "dom (flow_lookup \<u>_impl) = \<E>" "(\<forall> e \<in> 
   using  u_impl_exists[simplified sym[OF some_eq_ex]] 
   by (auto simp add: \<u>_impl_def) 
 
-lemma flow_network_impl:"flow_network (prod.fst \<circ> make_pair) (prod.snd \<circ> make_pair) make_pair create_edge (the_default PInfty \<circ> flow_lookup \<u>_impl) \<E>"
-proof -
-  have "snd = prod.snd \<circ> make_pair \<and> fst = prod.fst \<circ> make_pair"
-    by (auto simp add: make_pair''(1) make_pair''(2))
-  then show "flow_network (prod.fst \<circ> make_pair) (prod.snd \<circ> make_pair) make_pair create_edge (the_default PInfty \<circ> flow_lookup \<u>_impl) \<E>"
-    using flow_network_axioms \<u>_impl_props(1,2)
-    by(force split: option.split simp add:  flow_network_def flow_network_axioms_def the_default_def dom_def)
-qed
+lemma flow_network_impl:"flow_network fst snd create_edge (the_default PInfty \<circ> flow_lookup \<u>_impl) \<E>"
+ using flow_network_axioms \<u>_impl_props(1,2)
+ by(force split: option.split simp add:  flow_network_def flow_network_axioms_def the_default_def dom_def)
 
-lemma flow_network2:"flow_network (prod.fst \<circ> make_pair) (prod.snd \<circ> make_pair) make_pair create_edge \<u> \<E>"
-  using finite_E  by(auto intro!: flow_network.intro multigraph.intro flow_network_axioms.intro 
-                           simp add: create_edge E_not_empty u_non_neg)
+lemma flow_network2:"flow_network fst snd create_edge \<u> \<E>"
+  using finite_E  
+  by(auto intro!: flow_network.intro multigraph.intro flow_network_axioms.intro 
+        simp add: create_edge' E_not_empty u_non_neg)
 
 lemma b_impl_exists: "\<exists> b_impl. dom (bal_lookup b_impl) = \<V>  \<and> 
                          (\<forall> v \<in> \<V>. bal_lookup b_impl v = Some (b v)) \<and> bal_invar b_impl"
@@ -292,38 +280,37 @@ lemma b_impl_props: "dom (bal_lookup (b_impl b)) = \<V> " "(\<forall> v \<in> \<
   using  b_impl_exists[simplified sym[OF some_eq_ex]] 
   by (auto simp add: b_impl_def) force
 
-lemma solve_maxflow_proofs: "solve_maxflow_proofs s t make_pair create_edge \<E>_impl \<u>_impl \<E> (the_default PInfty \<circ> flow_lookup \<u>_impl)"
+lemma solve_maxflow_proofs: "solve_maxflow_proofs s t fst snd create_edge \<E>_impl \<u>_impl \<E> (the_default PInfty \<circ> flow_lookup \<u>_impl)"
   apply(rule solve_maxflow_proofs.intro[OF flow_network_impl], rule solve_maxflow_proofs_axioms.intro)
   by(auto simp add: \<E>_impl_prop \<u>_impl_props set_invar_def to_set_def s_in_V t_in_V s_neq_t)
 
 
 interpretation algo_locale: solve_maxflow_proofs
-  where  make_pair = make_pair and create_edge = create_edge
+  where  fst = fst and snd = snd and create_edge = create_edge
   and \<E>_impl = \<E>_impl and \<u>_impl = \<u>_impl and \<E> = \<E>
   and \<u> = "the_default PInfty \<circ> flow_lookup \<u>_impl" 
   using solve_maxflow_proofs by simp
 
 lemma algo_locale_isbflow_def:"algo_locale.isbflow f b =
-                   flow_network_spec.isbflow (prod.fst o make_pair) (prod.snd o make_pair)
-                                 make_pair \<E> (the_default PInfty \<circ> flow_lookup \<u>_impl) f b"
+                   flow_network_spec.isbflow fst snd \<E> (the_default PInfty \<circ> flow_lookup \<u>_impl) f b"
   by auto
 
 lemma to_maxflow_from_algo: "algo_locale.is_s_t_flow f s t \<Longrightarrow> f is s--t flow"
 proof(goal_cases)
   case 1
   hence all_props:"algo_locale.isuflow f" "algo_locale.ex f s \<le> 0"
-        "s \<in> algo_locale.\<V>" "t \<in> algo_locale.\<V>" "s \<noteq> t" 
-        "(\<And> x. x\<in>algo_locale.\<V> \<Longrightarrow> x \<noteq> s \<Longrightarrow> x \<noteq> t \<Longrightarrow> algo_locale.ex f x = 0)"
+        "s \<in> \<V>" "t \<in> \<V>" "s \<noteq> t" 
+        "(\<And> x. x\<in>\<V> \<Longrightarrow> x \<noteq> s \<Longrightarrow> x \<noteq> t \<Longrightarrow> algo_locale.ex f x = 0)"
     using algo_locale.is_s_t_flow_def[of f s t] by auto
   have "isuflow f"
     using all_props(1) \<u>_impl_props(2) 
     by(subst (asm)  algo_locale.isuflow_def )(auto simp add:  isuflow_def the_default_def)
   moreover have "ex f s \<le> 0"
     using all_props(2) \<u>_impl_props(2) 
-     by (auto simp add: algo_locale.ex_def   algo_locale.delta_minus_def algo_locale.delta_plus_def make_pair'' ex_def delta_plus_def delta_minus_def)
+     by (auto simp add: algo_locale.ex_def  delta_minus_def delta_plus_def  ex_def delta_plus_def delta_minus_def)
    moreover have "(\<And> x. x\<in>\<V> \<Longrightarrow> x \<noteq> s \<Longrightarrow> x \<noteq> t \<Longrightarrow> ex f x = 0)"
      using all_props(6)
-   by (auto simp add: algo_locale.ex_def   algo_locale.delta_minus_def algo_locale.delta_plus_def make_pair'' ex_def delta_plus_def delta_minus_def)
+   by (auto simp add: algo_locale.ex_def delta_minus_def delta_plus_def  ex_def delta_plus_def delta_minus_def)
   ultimately show ?case
     using s_in_V t_in_V s_neq_t by(auto intro!: is_s_t_flowI)
 qed
@@ -339,21 +326,21 @@ proof(goal_cases)
     by(subst  algo_locale.isuflow_def )(auto simp add:  isuflow_def the_default_def)
   moreover have "algo_locale.ex f s \<le> 0"
     using all_props(2) \<u>_impl_props(2) 
-     by (auto simp add: algo_locale.ex_def   algo_locale.delta_minus_def algo_locale.delta_plus_def make_pair'' ex_def delta_plus_def delta_minus_def)
+     by (auto simp add: delta_minus_def delta_plus_def ex_def )
    moreover have "(\<And> x. x\<in>\<V> \<Longrightarrow> x \<noteq> s \<Longrightarrow> x \<noteq> t \<Longrightarrow> algo_locale.ex f x = 0)"
      using all_props(6)
-   by (auto simp add: algo_locale.ex_def   algo_locale.delta_minus_def algo_locale.delta_plus_def make_pair'' ex_def delta_plus_def delta_minus_def)
+   by (auto simp add: ex_def delta_plus_def delta_minus_def)
   ultimately show ?case
     using s_in_V t_in_V s_neq_t flow_network_impl 
     by(auto intro!: flow_network_spec.is_s_t_flowI)
 qed
-
+term "(\<lambda>x. (if (x = s) then 0 else 0))"
 lemma existence_of_maximum_flow:
 "(\<exists> f. is_max_flow s t f) \<longleftrightarrow>  no_infty_path"
 proof(rule, goal_cases)
   case 1
   then obtain f where isopt: " is_max_flow s t f" by auto
-  define b where "b = (\<lambda>x. if x = s then ex\<^bsub>f\<^esub> t else if x = t then - ex\<^bsub>f\<^esub> t else 0)"
+  define b where "b = (\<lambda>x. (if (x = s) then (ex f t) else ( if (x = t) then (- ex f t) else 0)))"
   hence fbflow:"f is s--t flow" "f is b flow"
     using isopt is_max_flow_def s_t_flow_is_ex_bflow  by blast+
   moreover have no_infty_path
@@ -367,7 +354,7 @@ proof(rule, goal_cases)
       using 1(1) 
       by (auto simp add:  Rcap_def)
     have same_path:"(map (to_vertex_pair \<circ> F) D) = (map make_pair D)" 
-      by simp
+      by (simp add: make_pair_def Instantiation.make_pair_def)
     have fstv_is: "fstv (hd (map F D)) = s"
       using Dlen awalk_hd[OF u_prop(1)]
       by(cases D)(auto simp add:  make_pair'')
@@ -406,7 +393,7 @@ proof(rule, goal_cases)
         using after_augment isbflow_def by blast
     next
       case 2
-      have "ex\<^bsub>augment_edges f (real_of_ereal (min 1 (Rcap f (set ds)))) ds\<^esub> s = 
+      have "ex (augment_edges f (real_of_ereal (min 1 (Rcap f (set ds)))) ds) s = 
            - (b s + (real_of_ereal (min 1 (Rcap f (set ds)))))"
         using after_augment s_in_V ds_prop(4) fstv_is 
         by(fastforce simp add: isbflow_def)
@@ -420,7 +407,7 @@ proof(rule, goal_cases)
      finally show ?case by simp
     next
       case (3 x)
-      have "ex\<^bsub>augment_edges f (real_of_ereal (min 1 (Rcap f (set ds)))) ds\<^esub> x = 
+      have "ex (augment_edges f (real_of_ereal (min 1 (Rcap f (set ds)))) ds) x = 
             ex f x"
         using after_augment 3 t_in_V ds_prop(4,5) sndv_is s_neq_t fstv_is fbflow(2)
         by(fastforce simp add: isbflow_def)
@@ -428,17 +415,17 @@ proof(rule, goal_cases)
         using "3"(1) "3"(2) "3"(3) fbflow(1) is_s_t_flow_def by blast
       ultimately show ?case by simp
     qed
-    moreover have "ex\<^bsub>augment_edges f (real_of_ereal (min 1 (Rcap f (set ds)))) ds\<^esub> t
+    moreover have "ex (augment_edges f (real_of_ereal (min 1 (Rcap f (set ds)))) ds) t
                    > ex f t"
     proof-
-       have "ex\<^bsub>augment_edges f (real_of_ereal (min 1 (Rcap f (set ds)))) ds\<^esub> t =
+       have "ex (augment_edges f (real_of_ereal (min 1 (Rcap f (set ds)))) ds) t =
            - (b t - (real_of_ereal (min 1 (Rcap f (set ds)))))"
         using after_augment s_in_V ds_prop(4,5) fstv_is  s_neq_t sndv_is t_in_V by (auto simp add: isbflow_def)
       moreover  have "... > - b t" 
         using g_gtr_0 by argo
       moreover have "- b t = ex f t"
         using b_def fbflow(1) s_t_flow_excess_s_t by force
-      ultimately show "ex\<^bsub>augment_edges f (real_of_ereal (min 1 (Rcap f (set ds)))) ds\<^esub> t > ex f t"
+      ultimately show "ex (augment_edges f (real_of_ereal (min 1 (Rcap f (set ds)))) ds) t > ex f t"
         by simp
     qed
     ultimately show ?case 
@@ -461,35 +448,16 @@ next
     ultimately show ?case 
       using no_infty_path by blast
   qed
-  have success:"return (solve_maxflow.final_state_maxflow make_pair create_edge \<E>_impl \<u>_impl s t) = success"
+  have success:"return (solve_maxflow.final_state_maxflow fst snd create_edge \<E>_impl \<u>_impl s t) = success"
     using algo_locale.correctness_of_implementation(2,3)[OF no_infty_path'] return.exhaust by blast
   have max_flow_algo:"algo_locale.is_max_flow s t
- (abstract_flow_map (solve_maxflow.final_flow_impl_maxflow_original make_pair create_edge \<E>_impl \<u>_impl s t))"
+ (abstract_flow_map (solve_maxflow.final_flow_impl_maxflow_original fst snd create_edge \<E>_impl \<u>_impl s t))"
     using algo_locale.correctness_of_implementation(1)[OF no_infty_path' success] by simp
   have "is_max_flow s t
- (abstract_flow_map (solve_maxflow.final_flow_impl_maxflow_original make_pair create_edge \<E>_impl \<u>_impl s t))"
-  proof(rule is_max_flowI, goal_cases)
-    case 1
-    have "algo_locale.is_s_t_flow (abstract_flow_map 
-           (solve_maxflow.final_flow_impl_maxflow_original make_pair create_edge \<E>_impl \<u>_impl s t)) s t"
-      using max_flow_algo by(subst(asm) algo_locale.is_max_flow_def) simp
-    thus ?case
-      by(auto intro: to_maxflow_from_algo)
-    case (2 g)
-    hence "algo_locale.is_s_t_flow g s t"
-      by(force intro!: to_alog_max_flow) 
-    hence "algo_locale.ex g t \<le> algo_locale.ex (abstract_flow_map
-                (solve_maxflow.final_flow_impl_maxflow_original make_pair create_edge \<E>_impl \<u>_impl s t)) t"
-      using algo_locale.is_max_flow_def max_flow_algo s_in_V s_neq_t t_in_V by blast
-    moreover have "algo_locale.ex g t = ex g t"
-       by (auto simp add: algo_locale.ex_def algo_locale.delta_minus_def algo_locale.delta_plus_def make_pair'' ex_def delta_plus_def delta_minus_def)
-     moreover have " algo_locale.ex (abstract_flow_map
-                (solve_maxflow.final_flow_impl_maxflow_original make_pair create_edge \<E>_impl \<u>_impl s t)) t
-             =  ex (abstract_flow_map
-                (solve_maxflow.final_flow_impl_maxflow_original make_pair create_edge \<E>_impl \<u>_impl s t)) t"
-       by (auto simp add: algo_locale.ex_def algo_locale.delta_minus_def algo_locale.delta_plus_def make_pair'' ex_def delta_plus_def delta_minus_def)   
-    ultimately show ?case by auto
-  qed
+ (abstract_flow_map (solve_maxflow.final_flow_impl_maxflow_original fst snd create_edge \<E>_impl \<u>_impl s t))"
+    using  max_flow_algo to_alog_max_flow
+        to_maxflow_from_algo
+    by(auto elim!: flow_network_spec.is_max_flowE intro!: is_max_flowI)
   thus ?case by auto
 qed
 end
